feat: broadcast basic

src/Std/Sync/Broadcast.lean
@@ -12,8 +12,6 @@ public import Init.Data.Queue
 public import Std.Sync.Mutex
 public import Std.Internal.Async.Select
 
-public section
-
 /-!
 This module contains the implementation of `Std.Broadcast`. `Std.Broadcast` provides a
 broadcasting primitive for sending values to multiple consumers. It maintains a queue of
@@ -21,66 +19,350 @@ values and supports both synchronous and asynchronous waiting.
 -/
 
 namespace Std
-namespace CloseableBroadcast
 
 inductive Error where
   | closed
   | alreadyClosed
+  | noSubscribers
 
 instance : ToString Error where
   toString
     | .closed => "trying to send on an already closed channel"
     | .alreadyClosed => "trying to close an already closed broadcast channel"
+    | .noSubscribers => "there are no subscribers"
 
 instance : MonadLift (EIO Error) IO where
   monadLift x := EIO.toIO (.userError <| toString ·) x
 
 open Internal.IO.Async in
 
-private inductive Bounded.Consumer (α : Type) where
-  | normal (promise : IO.Promise (Option α))
-  | select (finished : Waiter (Option α))
+/--
 
-private def Bounded.Consumer.resolve (c : Consumer α) (x : Option α) : BaseIO Bool := do
-  match c with
-  | .normal promise =>
-    promise.resolve x
-    return true
-  | .select waiter =>
-    let lose := return false
-    let win promise := do
-      promise.resolve (.ok x)
-      return true
-    waiter.race lose win
+-/
+structure Broadcast.Consumer (α : Type) where
+  promise : IO.Promise Bool
+  waiter : Option (Waiter (Option α))
 
--- ??
+/--
 
+-/
+def Broadcast.Consumer.resolve (c : Broadcast.Consumer α) (b : Bool) : BaseIO Unit :=
+  c.promise.resolve b
+
+/--
+
+-/
 private structure Slot (α : Type) where
-  value : α
-  remaining : Mutex Nat
+  value : Option α
+  pos : Nat
+  remaining : Nat
+deriving Nonempty, Inhabited, Repr
 
-private structure Bounded.State (α : Type) where
+/--
+State of the channel.
+-/
+structure Broadcast.State (α : Type) where
+
+  /--
+  Producers that are waiting for a chance to write because the buffer is full.
+  -/
   producers : Std.Queue (IO.Promise Bool)
-  waiters : Std.Queue (Bounded.Consumer α)
 
-  buffer : CircularBuffer.Mutable α
+  /--
+  Consumers that are waiting for a chance to receive the last available value, because
+  they consumed all the ones that were available.
+  -/
+  waiters : Std.Queue (Broadcast.Consumer α)
 
-  receivers : Std.TreeSet Nat
+  /--
+  The capacity of the entire buffer.
+  -/
+  capacity : { x : Nat // x > 0 }
+
+  /--
+  The size of the entire buffer.
+  -/
+  size : Nat
+
+  /--
+  Circular buffer for storing the data that was sent.
+  -/
+  public buffer : Vector (IO.Ref (Slot α)) capacity
+
+  /--
+  The write pointer of the buffer
+  -/
+  write : Fin capacity
+
+  /--
+  The write pointer of the buffer
+  -/
+  read : Fin capacity
+
+  /--
+  Map from id to index.
+  -/
+  receivers : Std.TreeMap Nat Nat
+
+  /--
+  The next id for the next receiver
+  -/
   nextId : Nat
 
+  /--
+  Flag if the channel is closed.
+  -/
   closed : Bool
 
-private structure Bounded (α : Type) where
-  state : Mutex (Bounded.State α)
+  /--
+  Position
+  -/
+  pos : Nat
 
-private structure Bounded.Receiver (α : Type) where
-  state : Mutex (Bounded.State α)
-  next : Nat
+  /--
+  Mask
+  -/
+  mask : Nat
 
-namespace Bounded
+/--
+A channel that can create `Broadcast.Receiver` and send messages.
+-/
+structure ClosableBroadcast (α : Type) where
+  state : Mutex (Broadcast.State α)
 
-def subscribe (bounded : Bounded α) : IO (Receiver α) :=
-  sorry
+/--
+A channel that can receive messages from `Broadcast`.
+-/
+structure ClosableBroadcast.Receiver (α : Type) where
+  state : Mutex (Broadcast.State α)
+  id : Nat
 
-end Bounded
-end CloseableBroadcast
+/--
+A channel that can create `Broadcast.Receiver` and send messages.
+-/
+public def Broadcast := ClosableBroadcast
+
+
+/--
+A channel that can receive messages from `Broadcast`.
+-/
+public def Broadcast.Receiver := ClosableBroadcast.Receiver
+
+namespace Broadcast
+
+def bitLength : Nat → Nat
+  | 0 => 0
+  | n + 1 => 1 + bitLength ((n + 1) / 2)
+
+def nextPowerOfTwo (n : Nat) : Nat :=
+  if n = 0 then 0
+  else if n = 1 then 1
+  else 1 <<< (bitLength (n - 1))
+
+theorem shiftLeft_pos (m : Nat) : 1 <<< m > 0 := by
+  rw [Nat.shiftLeft_eq]
+  simp only [Nat.one_mul]
+  exact Nat.pow_pos (by decide)
+
+theorem nextPowerOfTwo_gt_zero_when_pos : n > 0 → nextPowerOfTwo n > 0 := by
+  intro h
+  simp [nextPowerOfTwo]
+  split
+  · omega
+  · split
+    · decide
+    · exact shiftLeft_pos _
+
+/--
+Creates a new `Broadcast` Channel.
+-/
+public def new (capacity : Nat := 16) (h : capacity > 0 := by decide) : BaseIO (Broadcast α) := do
+  let capacity := nextPowerOfTwo capacity
+
+  return { state := ← Mutex.new {
+    producers := .empty
+    waiters := .empty
+    buffer := ← Vector.mapM (fun _ => IO.mkRef { pos := 0, value := none, remaining := 0 }) (Vector.replicate capacity ())
+    receivers := .empty
+    nextId := 0
+    closed := false
+    pos := 0
+    size := 0
+    mask := capacity - 1
+    read := ⟨0, nextPowerOfTwo_gt_zero_when_pos h⟩
+    write := ⟨0, nextPowerOfTwo_gt_zero_when_pos h⟩
+    capacity := ⟨capacity, nextPowerOfTwo_gt_zero_when_pos h⟩
+  }}
+
+/--
+Subscribes a new `Receiver` in the `Broadcast` channel.
+-/
+public def subscribe (bd : Broadcast α) : IO (Receiver α) := do
+  let id ← bd.state.atomically do
+    modifyGet fun state =>
+      let id := state.nextId
+      (id, { state with nextId := id + 1, receivers := state.receivers.insert id state.pos })
+  return { state := bd.state, id }
+
+/-- Returns true if the buffer contains no elements. -/
+def isEmpty [Monad m] [MonadLiftT (ST IO.RealWorld) m] [MonadLiftT IO m] [MonadLiftT BaseIO m] : AtomicT (Broadcast.State α) m Bool := do
+  let mut st ← get
+  return st.size = 0
+
+/-- Returns true if the buffer is at full capacity. -/
+def isFull : AtomicT (Broadcast.State α) BaseIO Bool := do
+  let mut st ← get
+  return st.size ≥ st.capacity
+
+/--
+Enqueues an element to the back of the circular buffer.
+If the buffer is full, the oldest element (at front) is overwritten.
+-/
+def enqueue [Nonempty α] (value : α) (st : Broadcast.State α) : BaseIO (Broadcast.State α) := do
+  let tailRef := st.buffer.get st.write
+
+  tailRef.set { pos := st.pos, remaining := st.receivers.size, value := some value }
+
+  let size := st.size + 1
+  let write : Fin st.capacity := @Fin.ofNat _ ⟨Nat.ne_zero_iff_zero_lt.mpr st.capacity.property⟩ (st.write + 1)
+
+  return { st with write, size, pos := st.pos + 1 }
+
+/--
+Dequeues an element from the front of the circular buffer.
+Returns none if the buffer is empty.
+-/
+private def dequeue (st: State α) : State α :=
+    let size := st.size - 1
+    let read : Fin st.capacity := @Fin.ofNat _ ⟨Nat.ne_zero_iff_zero_lt.mpr st.capacity.property⟩ (st.read + 1)
+
+    { st with read, size }
+
+/--
+Peeks at the element at the front of the buffer without removing it.
+Returns none if the buffer is empty.
+-/
+def getSlot
+  [Monad m] [MonadLiftT (ST IO.RealWorld) m] [MonadLiftT IO m] [MonadLiftT BaseIO m] (place : Nat) :
+  AtomicT (Broadcast.State α) m (IO.Ref (Slot α)) := do
+    let mut st ← get
+    let idx := (@Fin.ofNat st.capacity ⟨Nat.ne_zero_of_lt st.capacity.property⟩ place)
+    return st.buffer.get idx
+
+/--
+Subscribes a new `Receiver` in the `Broadcast` channel.
+-/
+def trySend' [Nonempty α] (v : α) : AtomicT (Broadcast.State α) BaseIO Bool := do
+  if ← isFull then
+    return false
+  else
+    let mut st ← enqueue v (← get)
+    let mut waiters := st.waiters
+    set ({ st with waiters := ∅ })
+
+    for consumer in waiters.toArray do
+      discard <| consumer.resolve true
+
+    return true
+
+def trySend [Nonempty α] (ch : Broadcast α) (v : α) : BaseIO Bool := do
+  ch.state.atomically do
+    if (← get).closed then
+      return false
+    else
+      trySend' v
+
+public partial def send [Nonempty α] (ch : Broadcast α) (v : α) : BaseIO (Task (Except Error Unit)) := do
+  ch.state.atomically do
+    if (← get).closed then
+      return .pure <| .error .closed
+    else if (← get).receivers.isEmpty then
+      return .pure <| .error .noSubscribers
+    else if ← trySend' v then
+      return .pure <| .ok ()
+    else
+      let promise ← IO.Promise.new
+      modify fun st => { st with producers := st.producers.enqueue promise }
+
+      BaseIO.bindTask promise.result? fun res => do
+        if res.getD false then
+          Broadcast.send ch v
+        else
+          return .pure <| .error .closed
+
+def close (ch : Broadcast α) : EIO Error Unit := do
+  ch.state.atomically do
+    let st ← get
+
+    if st.closed then
+      throw .alreadyClosed
+
+    for consumer in st.waiters.toArray do
+      consumer.resolve false
+
+    set { st with waiters := ∅, closed := true }
+    return ()
+
+def isClosed (ch : Broadcast α) : BaseIO Bool :=
+  ch.state.atomically do
+    return (← get).closed
+
+
+namespace Receiver
+
+def getSlotValue
+  [Monad m] [MonadLiftT (ST IO.RealWorld) m] [MonadLiftT IO m] [MonadLiftT BaseIO m]
+  (slot : IO.Ref (Slot α)) (next : Nat) : AtomicT (Broadcast.State α) m (Option α × Bool) :=
+    slot.modifyGet fun slot =>
+      if next != slot.pos then
+        ((none, false), slot)
+      else if slot.remaining == 1 then
+        ((slot.value, true), { slot with value := none, remaining := 0 })
+      else
+        ((slot.value, false), { slot with remaining := slot.remaining - 1 })
+
+def tryRecv'
+  [Monad m] [MonadLiftT (ST IO.RealWorld) m] [MonadLiftT IO m] [MonadLiftT BaseIO m]
+  (receiverId : Nat) : AtomicT (Broadcast.State α) m (Option α) := do
+    let mut st ← get
+
+    if ← isEmpty then
+      return none
+
+    let next := st.receivers.get! receiverId
+    let id := next &&& st.mask
+
+    let slot ← getSlot id
+
+    let (some val, shouldDequeue) ← getSlotValue slot next
+      | return none
+
+    if shouldDequeue then
+      st := dequeue st
+
+      if let some (producer, producers) := st.producers.dequeue? then
+        producer.resolve true
+        st := { st with producers }
+
+    set { st with receivers := st.receivers.modify receiverId (· + 1) }
+
+    return some val
+
+def tryRecv (ch : Broadcast.Receiver α) : IO (Option α) :=
+  ch.state.atomically do
+    tryRecv' ch.id
+
+public partial def recv (ch : Broadcast.Receiver α) : IO (Task (Except IO.Error (Option α))) := do
+  ch.state.atomically do
+    if let some val ← tryRecv' ch.id then
+      return .pure <| .ok <| some val
+    else if (← get).closed then
+      return .pure <| .ok none
+    else
+      let promise ← IO.Promise.new
+      modify fun st => { st with waiters := st.waiters.enqueue ⟨promise, none⟩ }
+      IO.bindTask promise.result? fun res => do
+        if res.getD false then
+          Broadcast.Receiver.recv ch
+        else
+          return .pure (.ok none)
